<?xml version="1.0"?>


<!DOCTYPE rdf:RDF [
    <!ENTITY pav "http://purl.org/pav/" >
    <!ENTITY dct "http://purl.org/dc/terms/" >
    <!ENTITY prov "http://www.w3.org/ns/prov#" >
    <!ENTITY foaf "http://xmlns.com/foaf/0.1/" >
    <!ENTITY owl "http://www.w3.org/2002/07/owl#" >
    <!ENTITY dc "http://purl.org/dc/elements/1.1/" >
    <!ENTITY xsd "http://www.w3.org/2001/XMLSchema#" >
    <!ENTITY authoring "http://purl.org/pav/authoring/2.0/" >
    <!ENTITY versioning "http://purl.org/pav/versioning/2.0/" >
    <!ENTITY provenance "http://purl.org/pav/provenance/2.0/" >
    <!ENTITY rdfs "http://www.w3.org/2000/01/rdf-schema#" >
    <!ENTITY rdf "http://www.w3.org/1999/02/22-rdf-syntax-ns#" >
    <!ENTITY pav1 "http://swan.mindinformatics.org/ontologies/1.2/pav/" >
]>


<rdf:RDF xmlns="&pav;2.0/"
     xml:base="&pav;2.0/"
     xmlns:dc="http://purl.org/dc/elements/1.1/"
     xmlns:prov="http://www.w3.org/ns/prov#"
     xmlns:foaf="http://xmlns.com/foaf/0.1/"
     xmlns:versioning="&pav;versioning/2.0/"
     xmlns:provenance="&pav;provenance/2.0/"
     xmlns:pav1="http://swan.mindinformatics.org/ontologies/1.2/pav/"
     xmlns:rdfs="http://www.w3.org/2000/01/rdf-schema#"
     xmlns:pav="http://purl.org/pav/"
     xmlns:authoring="&pav;authoring/2.0/"
     xmlns:dct="http://purl.org/dc/terms/"
     xmlns:xsd="http://www.w3.org/2001/XMLSchema#"
     xmlns:owl="http://www.w3.org/2002/07/owl#"
     xmlns:rdf="http://www.w3.org/1999/02/22-rdf-syntax-ns#">
    <owl:Ontology rdf:about="http://purl.org/pav/">
        <rdfs:label xml:lang="en">Provenance, Authoring and Versioning (PAV)</rdfs:label>
        <owl:versionInfo rdf:datatype="&xsd;string">2.1</owl:versionInfo>
        <dct:modified rdf:datatype="&xsd;dateTime">2013-01-09T12:29:35+01:00</dct:modified>
        <dc:contributor rdf:datatype="&xsd;string">Marco Ocana</dc:contributor>
        <dc:creator rdf:datatype="&xsd;string">Paolo Ciccarese</dc:creator>
        <dc:contributor rdf:datatype="&xsd;string">Stian Soiland-Reyes</dc:contributor>
        <dct:format rdf:datatype="&xsd;string">application/rdf+xml</dct:format>
        <dct:language rdf:datatype="&xsd;language">en</dct:language>
        <dct:issued rdf:datatype="&xsd;dateTime">notyet</dct:issued>
        <dct:title xml:lang="en">PAV - Provenance, Authoring and Versioning</dct:title>
        <rdfs:comment xml:lang="en">PAV is a lightweight ontology for tracking Provenance, Authoring and Versioning. PAV specializes the W3C provenance ontology PROV-O in order to describe authorship, curation and digital creation of online resources.

This ontology describes the defined PAV properties and their usage. Note that PAV does not define any explicit classes or domain/ranges, as every property is meant to be used directly on the described online resource.</rdfs:comment>
        <dc:description xml:lang="en">PAV supplies terms for distinguishing between the different roles of the agents contributing content in current web based systems: contributors, authors, curators and digital artifact creators. The ontology also provides terms for tracking provenance of digital entities that are published on the web and then accessed, transformed and consumed. In order to support broader interoperability, PAV specializes the general purpose W3C PROV provenance model (PROV-O).

PAV distinguishes between the data related to the digital artifact - named Provenance - and those related to the actual knowledge creation and therefore to the intellectual property aspects â€“ named Authoring. The Versioning axis describes the evolution of digital entities in time. 

Using PAV, descriptions can define the Authors that originate or gave existence to the work that is expressed in the digital resource (pav:authoredBy); curators (pav:curatedBy) who are content specialists responsible for shaping the expression in an appropriate format, and contributors (super-property pav:contributedBy) that provided some help in conceiving the resource or in the expressed knowledge creation/extraction.

These provenance aspects can be detailed with dates using pav:curatedOn, pav:authoredOn, etc. Further details about the creation activities, such as different authors contributing specific parts of the resource at different dates are out of scope for PAV and should be defined using vocabularies like PROV-O and additional intermediate entities to describe the different states. 

For resources based on other resources, PAV allows specification of direct retrieval (pav:retrievedFrom), import through transformations (pav:importedFrom) and sources that were merely consulted (pav:sourceAccessedAt). These aspects can also define the agents responsible using pav:retrievedBy, pav:importedBy and pav:sourceAccessedBy. Version information can be specified using pav:previousVersion and pav:version. 

The creation of the digital representation, for instance an RDF graph, can in many cases be different from the authorship of the knowledge, and in PAV this digital creation is specified using pav:createdBy, pav:createdWith and pav:createdOn. 

The goal of PAV is to provide a lightweight, straight forward way to give the essential information about authorship, provenance and versioning, and therefore these properties are described directly on the published resource. As such, PAV does not define any classes or restrict domain/ranges, as all properties are applicable to any online resource.</dc:description>
        <rdfs:seeAlso rdf:resource="http://code.google.com/p/pav-ontology/"/>
        <rdfs:seeAlso rdf:resource="http://pav-ontology.googlecode.com/svn/trunk/1.2/pav.owl"/>
        <owl:imports rdf:resource="http://pav-ontology.googlecode.com/svn/trunk/1.2/pav.owl"/>
        <owl:backwardCompatibleWith rdf:resource="&pav;2.0/"/>
        <owl:priorVersion rdf:resource="&pav;2.0/"/>
        <owl:versionIRI rdf:resource="&pav;2.1/"/>
        <owl:backwardCompatibleWith rdf:resource="&pav;authoring/2.0/"/>
        <owl:backwardCompatibleWith rdf:resource="&pav;provenance/2.0/"/>
        <owl:backwardCompatibleWith rdf:resource="&pav;versioning/2.0/"/>
        <dct:contributor rdf:resource="http://soiland-reyes.com/stian/#me"/>
        <dct:publisher rdf:resource="http://swan.mindinformatics.org/"/>
        <owl:incompatibleWith rdf:resource="http://swan.mindinformatics.org/ontologies/1.2/pav.owl"/>
        <dct:creator rdf:resource="http://www.hcklab.org/foaf.rdf#me"/>
        <dct:creator rdf:resource="http://www.paolociccarese.info/"/>
        <owl:imports rdf:resource="http://www.w3.org/ns/prov#"/>
        <rdfs:seeAlso rdf:resource="http://www.w3.org/ns/prov#"/>
    </owl:Ontology>
    


    <!-- 
    ///////////////////////////////////////////////////////////////////////////////////////
    //
    // Annotation properties
    //
    ///////////////////////////////////////////////////////////////////////////////////////
     -->

    


    <!-- 
    ///////////////////////////////////////////////////////////////////////////////////////
    //
    // Datatypes
    //
    ///////////////////////////////////////////////////////////////////////////////////////
     -->

    


    <!-- 
    ///////////////////////////////////////////////////////////////////////////////////////
    //
    // Object Properties
    //
    ///////////////////////////////////////////////////////////////////////////////////////
     -->

    


    <!-- http://purl.org/pav/authoredBy -->

    <owl:ObjectProperty rdf:about="&pav;authoredBy">
        <rdfs:label xml:lang="en">Authored by</rdfs:label>
        <rdfs:comment xml:lang="en">An agent that originated or gave existence to the work that is expressed by the digital resource.

The author of the content of a resource is different from the creator of that digital resource (although they are often the same). See pav:createdBy for a discussion.</rdfs:comment>
        <rdfs:subPropertyOf rdf:resource="&pav;contributedBy"/>
        <rdfs:seeAlso rdf:resource="&pav;createdBy"/>
        <owl:equivalentProperty rdf:resource="&pav1;authoredBy"/>
    </owl:ObjectProperty>
    


    <!-- http://purl.org/pav/contributedBy -->

    <owl:ObjectProperty rdf:about="&pav;contributedBy">
        <rdfs:label xml:lang="en">Contributed by</rdfs:label>
        <rdfs:comment xml:lang="en">An agent that provided any sort of help in conceiving the work that is expressed by the digital artifact.

The date of contribution can be expressed using pav:contributedOn - note however that there is no relationship in PAV identifying which contributor contributed when or what, such lineage should rather be expressed using a process-centric model such as OPM or PROV.

Note that as pav:contributedBy identifies only agents that contributed to the work, and not agents that made the digital artifact, it is more precise than dct:contributor. See pav:createdBy for a discussion.</rdfs:comment>
        <owl:equivalentProperty rdf:resource="&pav1;contributedBy"/>
        <rdfs:subPropertyOf rdf:resource="&prov;wasAttributedTo"/>
    </owl:ObjectProperty>
    


    <!-- http://purl.org/pav/createdAt -->

    <owl:ObjectProperty rdf:about="&pav;createdAt">
        <rdfs:label xml:lang="en">Created at</rdfs:label>
        <rdfs:comment xml:lang="en">The geo-location of the agent that created the annotation.</rdfs:comment>
        <rdfs:seeAlso rdf:resource="&pav;createdBy"/>
    </owl:ObjectProperty>
    


    <!-- http://purl.org/pav/createdBy -->

    <owl:ObjectProperty rdf:about="&pav;createdBy">
        <rdfs:label xml:lang="en">Created by</rdfs:label>
        <rdfs:comment xml:lang="en">An entity primary responsible for making the digital artifact.

This property is distinct from pav:authoredBy, which identifies who authored the knowledge expressed by this resource, and pav:curatedBy, which identifies who curated the knowledge into its current form. 

pav:createdBy is more specific than dct:createdBy - which might or might not be interpreted to cover this creator.

For instance, the author wrote &apos;this species has bigger wings than normal&apos; in his log book. The curator, going through the log book and identifying important knowledge, formalizes this as &apos;locus perculus has wingspan &gt; 0.5m&apos;. The creator enters this knowledge as a digital resource in the knowledge system, thus creating the digital artifact (say as JSON, RDF, XML or HTML).

A different example is a news article. pav:authoredBy indicates the journalist who wrote the article. pav:curatedBy can indicate the editor who made the article conform to the news paper&apos;s style. pav:createdBy can indicate who put the article on the web site.

The software tool used by the creator to make the digital resource (say Protege, Wordpress or OpenOffice) can be indicated with pav:createdWith.

The date the digital resource was created can be indicated with pav:createdOn.

The location the agent was when creating the digital resource can be made using pav:createdAt.</rdfs:comment>
        <rdfs:seeAlso rdf:resource="&pav;authoredBy"/>
        <rdfs:seeAlso rdf:resource="&pav;createdAt"/>
        <rdfs:seeAlso rdf:resource="&pav;createdOn"/>
        <rdfs:seeAlso rdf:resource="&pav;curatedBy"/>
        <owl:equivalentProperty rdf:resource="&pav1;createdBy"/>
        <rdfs:subPropertyOf rdf:resource="&prov;wasAttributedTo"/>
    </owl:ObjectProperty>
    


    <!-- http://purl.org/pav/createdWith -->

    <owl:ObjectProperty rdf:about="&pav;createdWith">
        <rdfs:label xml:lang="en">Created with</rdfs:label>
        <rdfs:comment xml:lang="en">The software/tool used by the creator when making the digital resource. 

For instance: Protege, Wordpress, LibreOffice.</rdfs:comment>
        <rdfs:seeAlso rdf:resource="&pav;createdBy"/>
        <rdfs:subPropertyOf rdf:resource="&prov;wasAttributedTo"/>
    </owl:ObjectProperty>
    


    <!-- http://purl.org/pav/curatedBy -->

    <owl:ObjectProperty rdf:about="&pav;curatedBy">
        <rdfs:label xml:lang="en">Curated by</rdfs:label>
        <rdfs:comment xml:lang="en">An agent specialist responsible for shaping the expression in an appropriate format. Often the primary agent responsible for ensuring the quality of the representation.

The curator is different from the creator of the digital resource (although they are often the same), see pav:createdBy for a discussion.</rdfs:comment>
        <rdfs:subPropertyOf rdf:resource="&pav;contributedBy"/>
        <rdfs:seeAlso rdf:resource="&pav;createdBy"/>
        <owl:equivalentProperty rdf:resource="&pav1;curatedBy"/>
    </owl:ObjectProperty>
    


    <!-- http://purl.org/pav/curates -->

    <owl:ObjectProperty rdf:about="&pav;curates">
        <rdfs:label xml:lang="en">Curates</rdfs:label>
        <owl:deprecated rdf:datatype="&xsd;boolean">true</owl:deprecated>
        <rdfs:comment xml:lang="en">Provided for backwards compatibility with PAV 1.2 only. Use instead the inverse pav:curatedBy.</rdfs:comment>
        <owl:inverseOf rdf:resource="&pav;curatedBy"/>
    </owl:ObjectProperty>
    


    <!-- http://purl.org/pav/derivedFrom -->

    <owl:ObjectProperty rdf:about="&pav;derivedFrom">
        <rdfs:label xml:lang="en">Derived from</rdfs:label>
        <rdfs:comment xml:lang="en">Derived from a different resource. Derivation conserns itself with derived knowledge. If this resource has the same content as the other resource, but has simply been transcribed to fit a different model (like XML -&gt; RDF or SQL -&gt; CVS), use pav:importedFrom. If the content has been further refined or modified, use pav:derivedFrom.</rdfs:comment>
        <rdfs:seeAlso rdf:resource="&pav;importedFrom"/>
        <rdfs:seeAlso rdf:resource="&pav;previousVersion"/>
        <rdfs:subPropertyOf rdf:resource="&prov;wasDerivedFrom"/>
    </owl:ObjectProperty>
    


    <!-- http://purl.org/pav/importedBy -->

    <owl:ObjectProperty rdf:about="&pav;importedBy">
        <rdfs:label xml:lang="en">Imported by</rdfs:label>
        <rdfs:comment xml:lang="en">An entity responsible for importing the data. 

The importer is usually a software entity which has done the transcription from the original source.

See pav:importedFrom for a discussion of import vs. retrieve vs. derived.</rdfs:comment>
        <rdfs:seeAlso rdf:resource="&pav;importedFrom"/>
        <owl:equivalentProperty rdf:resource="&pav1;importedBy"/>
        <rdfs:subPropertyOf rdf:resource="&prov;wasAttributedTo"/>
    </owl:ObjectProperty>
    


    <!-- http://purl.org/pav/importedFrom -->

    <owl:ObjectProperty rdf:about="&pav;importedFrom">
        <rdfs:label xml:lang="en">Imported from</rdfs:label>
        <rdfs:comment xml:lang="en">The original source of the imported information. 

Import means that the content has been preserved, but transcribed somehow, for instance to fit a different model. Examples of import are when the original was JSON and the current resource is RDF, or where the original was an document scan, and this resource is the text found through OCR. 

The difference between pav:derivedFrom and pav:importedFrom is that the imported resource conveys the same knowledge/content as the original, while a derived resource has somehow modified that knowledge to convey something else.

If the resource has been copied verbatim from the original (e.g. downloaded), use pav:retrievedFrom.

To indicate which agent(s) performed the import, use pav:importedBy. Use pav:importedOn to indicate when it happened.</rdfs:comment>
        <rdfs:seeAlso rdf:resource="&pav;derivedFrom"/>
        <rdfs:seeAlso rdf:resource="&pav;importedBy"/>
        <rdfs:seeAlso rdf:resource="&pav;importedOn"/>
        <rdfs:seeAlso rdf:resource="&pav;retrievedFrom"/>
        <owl:equivalentProperty rdf:resource="&pav1;importedFromSource"/>
        <rdfs:subPropertyOf rdf:resource="&prov;wasDerivedFrom"/>
    </owl:ObjectProperty>
    


    <!-- http://purl.org/pav/previousVersion -->

    <owl:ObjectProperty rdf:about="&pav;previousVersion">
        <rdfs:label xml:lang="en">Previous version</rdfs:label>
        <rdfs:comment xml:lang="en">The previous version of a resource in a lineage. For instance a news article updated to correct factual information would point to the previous version of the article with pav:previousVersion. If however the content has significantly changed so that the two resources no longer share lineage (say a new news article that talks about the same facts), they should be related using pav:derivedFrom.

A version number of this resource can be provided using the data property pav:version.</rdfs:comment>
        <rdfs:seeAlso rdf:resource="&pav;derivedFrom"/>
        <rdfs:seeAlso rdf:resource="&pav;version"/>
        <owl:equivalentProperty rdf:resource="&pav1;previousVersion"/>
        <rdfs:subPropertyOf rdf:resource="&prov;wasRevisionOf"/>
    </owl:ObjectProperty>
    


    <!-- http://purl.org/pav/providedBy -->

    <owl:ObjectProperty rdf:about="&pav;providedBy">
        <rdfs:label xml:lang="en">Provided by</rdfs:label>
        <rdfs:comment xml:lang="en">The provider of the encoded information (PubMed, UniProt, Science Commons). The provider might not coincide with the dct:publisher.</rdfs:comment>
        <rdfs:seeAlso rdf:resource="&dct;publisher"/>
    </owl:ObjectProperty>
    


    <!-- http://purl.org/pav/retrievedBy -->

    <owl:ObjectProperty rdf:about="&pav;retrievedBy">
        <rdfs:label xml:lang="en">Retrieved by</rdfs:label>
        <rdfs:comment xml:lang="en">An entity responsible for retrieving the data from an external source. 

The importer is usually a software entity which has done the retrieval from the original source without performing any transcription.

See pav:importedFrom for a discussion of import vs. retrieve vs. derived.</rdfs:comment>
        <rdfs:seeAlso rdf:resource="&pav;importedFrom"/>
        <rdfs:subPropertyOf rdf:resource="&prov;wasAttributedTo"/>
    </owl:ObjectProperty>
    


    <!-- http://purl.org/pav/retrievedFrom -->

    <owl:ObjectProperty rdf:about="&pav;retrievedFrom">
        <rdfs:label xml:lang="en">Retrieved from</rdfs:label>
        <rdfs:comment xml:lang="en">The URI where a resource has been retrieved from.

Retrieval indicates that this resource has the same representation as the original resource. If the resource has been somewhat transformed, use pav:importedFrom instead.

The time of the retrieval should be indicated using pav:retrievedOn. The agent may be indicated with pav:retrievedBy.</rdfs:comment>
        <rdfs:seeAlso rdf:resource="&pav;retrievedBy"/>
        <rdfs:seeAlso rdf:resource="&pav;retrievedOn"/>
        <rdfs:subPropertyOf rdf:resource="&prov;wasDerivedFrom"/>
    </owl:ObjectProperty>
    


    <!-- http://purl.org/pav/sourceAccessedAt -->

    <owl:ObjectProperty rdf:about="&pav;sourceAccessedAt">
        <rdfs:label xml:lang="en">Source accessed at</rdfs:label>
        <rdfs:comment xml:lang="en">A source which was accessed (but not retrieved or imported).</rdfs:comment>
        <rdfs:seeAlso rdf:resource="&pav;importedFrom"/>
        <rdfs:seeAlso rdf:resource="&pav;retrievedFrom"/>
        <rdfs:subPropertyOf rdf:resource="&prov;wasInfluencedBy"/>
    </owl:ObjectProperty>
    


    <!-- http://purl.org/pav/sourceAccessedBy -->

    <owl:ObjectProperty rdf:about="&pav;sourceAccessedBy">
        <rdfs:label xml:lang="en">Source accessed by</rdfs:label>
        <rdfs:comment xml:lang="en">The agent who accessed the source</rdfs:comment>
        <rdfs:seeAlso rdf:resource="&pav;sourceAccessedAt"/>
    </owl:ObjectProperty>
    


    <!-- http://swan.mindinformatics.org/ontologies/1.2/pav/authoredBy -->

    <rdf:Description rdf:about="&pav1;authoredBy"/>
    


    <!-- http://swan.mindinformatics.org/ontologies/1.2/pav/contributedBy -->

    <rdf:Description rdf:about="&pav1;contributedBy"/>
    


    <!-- http://swan.mindinformatics.org/ontologies/1.2/pav/createdBy -->

    <rdf:Description rdf:about="&pav1;createdBy"/>
    


    <!-- http://swan.mindinformatics.org/ontologies/1.2/pav/curatedBy -->

    <rdf:Description rdf:about="&pav1;curatedBy"/>
    


    <!-- http://swan.mindinformatics.org/ontologies/1.2/pav/importedBy -->

    <rdf:Description rdf:about="&pav1;importedBy"/>
    


    <!-- http://swan.mindinformatics.org/ontologies/1.2/pav/importedFromSource -->

    <rdf:Description rdf:about="&pav1;importedFromSource"/>
    


    <!-- http://swan.mindinformatics.org/ontologies/1.2/pav/previousVersion -->

    <rdf:Description rdf:about="&pav1;previousVersion"/>
    


    <!-- 
    ///////////////////////////////////////////////////////////////////////////////////////
    //
    // Data properties
    //
    ///////////////////////////////////////////////////////////////////////////////////////
     -->

    


    <!-- http://purl.org/pav/authoredOn -->

    <owl:DatatypeProperty rdf:about="&pav;authoredOn">
        <rdfs:label xml:lang="en">Authored on</rdfs:label>
        <rdfs:comment xml:lang="en">The date this resource was authored.

pav:authoredBy gives the authoring agent.

Note that pav:authoredOn is different from pav:createdOn, although they are often the same. See pav:createdBy for a discussion.</rdfs:comment>
        <rdfs:seeAlso rdf:resource="&pav;authoredBy"/>
        <rdfs:subPropertyOf rdf:resource="&pav;contributedOn"/>
        <rdfs:seeAlso rdf:resource="&pav;createdBy"/>
        <rdfs:seeAlso rdf:resource="&pav;createdOn"/>
    </owl:DatatypeProperty>
    


    <!-- http://purl.org/pav/contributedOn -->

    <owl:DatatypeProperty rdf:about="&pav;contributedOn">
        <rdfs:label xml:lang="en">Contributed on</rdfs:label>
        <rdfs:comment xml:lang="en">The date this resource was contributed to.

pav:contributedBy provides the agent that contributed.</rdfs:comment>
        <rdfs:seeAlso rdf:resource="&pav;contributedBy"/>
        <rdfs:range rdf:resource="&xsd;dateTime"/>
    </owl:DatatypeProperty>
    


    <!-- http://purl.org/pav/createdOn -->

    <owl:DatatypeProperty rdf:about="&pav;createdOn">
        <rdfs:label xml:lang="en">Created On</rdfs:label>
        <rdfs:comment xml:lang="en">The date of creation of the resource.</rdfs:comment>
        <rdfs:seeAlso rdf:resource="&pav;createdBy"/>
        <owl:equivalentProperty rdf:resource="&pav1;createdOn"/>
        <rdfs:range rdf:resource="&xsd;dateTime"/>
    </owl:DatatypeProperty>
    


    <!-- http://purl.org/pav/curatedOn -->

    <owl:DatatypeProperty rdf:about="&pav;curatedOn">
        <rdfs:label xml:lang="en">Curated on</rdfs:label>
        <rdfs:comment xml:lang="en">The date this resource was curated. 

pav:curatedBy gives the agents that performed the curation.</rdfs:comment>
        <rdfs:subPropertyOf rdf:resource="&pav;contributedOn"/>
        <rdfs:seeAlso rdf:resource="&pav;curatedBy"/>
    </owl:DatatypeProperty>
    


    <!-- http://purl.org/pav/importedOn -->

    <owl:DatatypeProperty rdf:about="&pav;importedOn">
        <rdfs:label xml:lang="en">Imported on</rdfs:label>
        <rdfs:comment xml:lang="en">The date this resource was imported.

See pav:importedFrom for a discussion about import vs. retrieval.</rdfs:comment>
        <rdfs:seeAlso rdf:resource="&pav;importedBy"/>
        <rdfs:seeAlso rdf:resource="&pav;importedFrom"/>
        <owl:equivalentProperty rdf:resource="&pav1;importedOn"/>
        <rdfs:range rdf:resource="&xsd;dateTime"/>
    </owl:DatatypeProperty>
    


    <!-- http://purl.org/pav/lastRefreshedOn -->

    <owl:DatatypeProperty rdf:about="&pav;lastRefreshedOn">
        <rdfs:label xml:lang="en">Last refreshed on</rdfs:label>
        <rdfs:comment xml:lang="en">The date of the last import of the resource. This property is used if this version has been updated due to a re-import, rather than the import creating new resources related using pav:previousVersion.</rdfs:comment>
        <rdfs:seeAlso rdf:resource="&pav;importedBy"/>
        <rdfs:seeAlso rdf:resource="&pav;importedFrom"/>
        <rdfs:seeAlso rdf:resource="&pav;importedOn"/>
        <rdfs:seeAlso rdf:resource="&pav;previousVersion"/>
        <owl:equivalentProperty rdf:resource="&pav1;importedLastOn"/>
        <rdfs:range rdf:resource="&xsd;dateTime"/>
    </owl:DatatypeProperty>
    


    <!-- http://purl.org/pav/lastUpdateOn -->

    <owl:DatatypeProperty rdf:about="&pav;lastUpdateOn">
        <rdfs:label xml:lang="en">Last updated on</rdfs:label>
        <rdfs:comment xml:lang="en">The date of the last update of the resource. An update is a change which did not warrant making a new resource related using pav:previousVersion, for instance correcting a spelling mistake.</rdfs:comment>
        <rdfs:seeAlso rdf:resource="&pav;createdOn"/>
        <rdfs:seeAlso rdf:resource="&pav;previousVersion"/>
        <owl:equivalentProperty rdf:resource="&pav1;lastUpdateOn"/>
        <rdfs:range rdf:resource="&xsd;dateTime"/>
    </owl:DatatypeProperty>
    


    <!-- http://purl.org/pav/retrievedOn -->

    <owl:DatatypeProperty rdf:about="&pav;retrievedOn">
        <rdfs:label xml:lang="en">Retrieved on</rdfs:label>
        <rdfs:comment xml:lang="en">The date this resource was retrieved. </rdfs:comment>
        <rdfs:seeAlso rdf:resource="&pav;retrievedBy"/>
        <rdfs:seeAlso rdf:resource="&pav;retrievedFrom"/>
        <rdfs:range rdf:resource="&xsd;dateTime"/>
    </owl:DatatypeProperty>
    


    <!-- http://purl.org/pav/sourceAccessedOn -->

    <owl:DatatypeProperty rdf:about="&pav;sourceAccessedOn">
        <rdfs:label xml:lang="en">Source accessed on</rdfs:label>
        <rdfs:comment xml:lang="en">The date when the original source has been accessed to create the resource.</rdfs:comment>
        <rdfs:seeAlso rdf:resource="&pav;createdAt"/>
        <rdfs:seeAlso rdf:resource="&pav;sourceAccessedAt"/>
        <rdfs:seeAlso rdf:resource="&pav;sourceAccessedBy"/>
        <owl:equivalentProperty rdf:resource="&pav1;sourceAccessedOn"/>
        <owl:equivalentProperty rdf:resource="&pav1;sourceFirstAccessedOn"/>
        <rdfs:range rdf:resource="&xsd;dateTime"/>
    </owl:DatatypeProperty>
    


    <!-- http://purl.org/pav/sourceLastAccessedOn -->

    <owl:DatatypeProperty rdf:about="&pav;sourceLastAccessedOn">
        <rdfs:label xml:lang="en">Source last accessed on</rdfs:label>
        <rdfs:comment xml:lang="en">The date when the original source has been last accessed and verified.</rdfs:comment>
        <rdfs:seeAlso rdf:resource="&pav;createdAt"/>
        <rdfs:seeAlso rdf:resource="&pav;sourceAccessedAt"/>
        <rdfs:seeAlso rdf:resource="&pav;sourceAccessedBy"/>
        <owl:equivalentProperty rdf:resource="&pav1;sourceLastAccessedOn"/>
        <rdfs:range rdf:resource="&xsd;dateTime"/>
    </owl:DatatypeProperty>
    


    <!-- http://purl.org/pav/version -->

    <owl:DatatypeProperty rdf:about="&pav;version">
        <rdfs:label xml:lang="en">Version</rdfs:label>
        <rdfs:comment rdf:datatype="&xsd;string">The version number of a resource. This is a freetext string, typical values are &quot;1.5&quot; or &quot;21&quot;. The URI identifying the previous version can be provided using prov:previousVersion.</rdfs:comment>
        <rdfs:seeAlso rdf:resource="&pav;previousVersion"/>
        <owl:equivalentProperty rdf:resource="&pav1;versionNumber"/>
        <rdfs:range rdf:resource="&xsd;string"/>
    </owl:DatatypeProperty>
    


    <!-- http://swan.mindinformatics.org/ontologies/1.2/pav/createdOn -->

    <rdf:Description rdf:about="&pav1;createdOn"/>
    


    <!-- http://swan.mindinformatics.org/ontologies/1.2/pav/importedLastOn -->

    <rdf:Description rdf:about="&pav1;importedLastOn"/>
    


    <!-- http://swan.mindinformatics.org/ontologies/1.2/pav/importedOn -->

    <rdf:Description rdf:about="&pav1;importedOn"/>
    


    <!-- http://swan.mindinformatics.org/ontologies/1.2/pav/lastUpdateOn -->

    <rdf:Description rdf:about="&pav1;lastUpdateOn"/>
    


    <!-- http://swan.mindinformatics.org/ontologies/1.2/pav/sourceAccessedOn -->

    <rdf:Description rdf:about="&pav1;sourceAccessedOn"/>
    


    <!-- http://swan.mindinformatics.org/ontologies/1.2/pav/sourceFirstAccessedOn -->

    <rdf:Description rdf:about="&pav1;sourceFirstAccessedOn"/>
    


    <!-- http://swan.mindinformatics.org/ontologies/1.2/pav/sourceLastAccessedOn -->

    <rdf:Description rdf:about="&pav1;sourceLastAccessedOn"/>
    


    <!-- http://swan.mindinformatics.org/ontologies/1.2/pav/versionNumber -->

    <rdf:Description rdf:about="&pav1;versionNumber"/>
</rdf:RDF>



<!-- Generated by the OWL API (version 3.3.1957) http://owlapi.sourceforge.net -->

